use new loop combinator in Frodo.Encode

frodo/code/Hacl.Impl.Frodo.Encode.fst
@@ -16,10 +16,8 @@ open Hacl.Impl.Frodo.Params
 
 module B  = LowStar.Buffer
 module ST = FStar.HyperStack.ST
-module HS = FStar.HyperStack
 
 module LSeq = Lib.Sequence
-module M    = Spec.Matrix
 module S    = Spec.Frodo.Encode
 module FLemmas = Spec.Frodo.Lemmas
 
@@ -31,7 +29,7 @@ val ec:
   -> k:uint16{uint_v k < pow2 (v b)}
   -> r:uint16{r == S.ec (v b) k}
 let ec b a =
-  a <<. (size_to_uint32 (params_logq -. b))
+  a <<. (params_logq -. b)
 
 inline_for_extraction noextract private
 val dc:
@@ -39,8 +37,8 @@ val dc:
   -> c:uint16
   -> r:uint16{r == S.dc (v b) c}
 let dc b c =
-  let res1 = (c +. (u16 1 <<. size_to_uint32 (params_logq -. b -. size 1))) >>. size_to_uint32 (params_logq -. b) in
-  res1 &. ((u16 1 <<. size_to_uint32 b) -. u16 1)
+  let res1 = (c +. (u16 1 <<. (params_logq -. b -. size 1))) >>. (params_logq -. b) in
+  res1 &. ((u16 1 <<. b) -. u16 1)
 
 inline_for_extraction noextract private
 val ec1:
@@ -49,151 +47,124 @@ val ec1:
   -> k:size_t{v k < 8}
   -> res:uint16{res == S.ec1 (v b) x (v k)}
 let ec1 b x k =
-  FLemmas.modulo_pow2_u64 (x >>. size_to_uint32 (b *! k)) (v b);
-  let rk = (x >>. size_to_uint32 (b *! k)) &. ((u64 1 <<. size_to_uint32 b) -. u64 1) in
+  FLemmas.modulo_pow2_u64 (x >>. (b *! k)) (v b);
+  let rk = (x >>. (b *! k)) &. ((u64 1 <<. b) -. u64 1) in
   ec b (to_u16 rk)
 
 inline_for_extraction noextract private
 val frodo_key_encode1:
     b:size_t{0 < v b /\ v b <= 8}
   -> a:lbytes (params_nbar *! params_nbar *! b /. size 8)
-  -> res0:matrix_t params_nbar params_nbar
-  -> vi:uint64
   -> i:size_t{v i < v params_nbar}
-  -> Stack unit
-    (requires fun h ->
-      B.live h a /\ B.live h res0 /\ B.disjoint a res0)
-    (ensures fun h0 _ h1 ->
-      B.live h1 res0 /\ modifies (loc_buffer res0) h0 h1 /\
-      as_matrix h1 res0 == S.frodo_key_encode1 (v b) (B.as_seq h0 a) (as_matrix h0 res0) vi (v i))
-let frodo_key_encode1 b a res0 vi i =
-  let h0 = ST.get () in
-  Lib.Loops.for (size 0) (size 8)
-  (fun h1 k ->
-    B.live h1 res0 /\ B.live h1 a /\ modifies (loc_buffer res0) h0 h1 /\
-    (forall (i0:size_nat{i0 < v params_nbar /\ i0 <> v i}) (k:size_nat{k < 8}).
-      get h1 res0 i0 k == get h0 res0 i0 k) /\
-    (forall (k1:size_nat{k1 < k}). get h1 res0 (v i) k1 == S.ec1 (v b) vi k1) /\
-    (forall (k1:size_nat{k <= k1 /\ k1 < 8}). get h1 res0 (v i) k1 == get h0 res0 (v i) k1))
-  (fun k ->
-    mset res0 i k (ec1 b vi k)
-  );
-  let h2 = ST.get () in
-  S.lemma_matrix_equality_nbar (as_matrix h2 res0) (S.frodo_key_encode1 (v b) (B.as_seq h0 a) (as_matrix h0 res0) vi (v i))
+  -> Stack uint64
+    (requires fun h -> B.live h a)
+    (ensures fun h0 r h1 ->
+      modifies loc_none h0 h1 /\
+      r == S.frodo_key_encode1 (v b) (as_seq h0 a) (v i))
+let frodo_key_encode1 b a i =
+  push_frame();
+  let v8 = create (size 8) (u8 0) in
+  update_sub v8 (size 0) b (sub #_ #_ #(v b) a (i *! b) b);
+  let x = uint_from_bytes_le #U64 v8 in
+  pop_frame();
+  x
 
 inline_for_extraction noextract private
 val frodo_key_encode2:
     b:size_t{0 < v b /\ v b <= 8}
   -> a:lbytes (params_nbar *! params_nbar *! b /. size 8)
-  -> res0:matrix_t params_nbar params_nbar
   -> i:size_t{v i < v params_nbar}
+  -> x:uint64
+  -> res:matrix_t params_nbar params_nbar
   -> Stack unit
-    (requires fun h -> B.live h a /\ B.live h res0 /\ B.disjoint a res0)
-    (ensures  fun h0 _ h1 ->
-      B.live h1 a /\ B.live h1 res0 /\
-      modifies (loc_buffer res0) h0 h1 /\
-      as_matrix h1 res0 == S.frodo_key_encode2 (v b) (B.as_seq h0 a) (as_matrix h0 res0) (v i))
-let frodo_key_encode2 b a res0 i =
-  push_frame();
-  let v8 = create (size 8) (u8 0) in
-  let aLen = params_nbar *! params_nbar *! b /. size 8 in
-  update_sub v8 (size 0) b (sub #_ #_ #(v b) a (i *! b) b);
-  let vi = uint_from_bytes_le #U64 v8 in
-  frodo_key_encode1 b a res0 vi i;
-  pop_frame()
-
-#set-options "--max_fuel 1"
+    (requires fun h ->
+      B.live h a /\ B.live h res /\ B.disjoint a res)
+    (ensures fun h0 _ h1 ->
+      modifies (loc_buffer res) h0 h1 /\
+      as_matrix h1 res == S.frodo_key_encode2 (v b) (as_seq h0 a) (v i) x (as_matrix h0 res))
+let frodo_key_encode2 b a i x res =
+  [@ inline_let]
+  let spec h0 = S.frodo_key_encode0 (v b) (as_seq h0 a) x (v i) in
+  let h0 = ST.get () in
+  loop1 h0 (size 8) res spec
+  (fun k ->
+    Lib.LoopCombinators.unfold_repeati 8 (spec h0) (as_seq h0 res) (v k);
+    mset res i k (ec1 b x k)
+  )
 
 val frodo_key_encode:
     b:size_t{0 < v b /\ v b <= 8}
   -> a:lbytes (params_nbar *! params_nbar *! b /. size 8)
   -> res:matrix_t params_nbar params_nbar
   -> Stack unit
-    (requires fun h -> B.live h a /\ B.live h res /\ B.disjoint a res)
-    (ensures  fun h0 _ h1 -> B.live h1 res /\ modifies (loc_buffer res) h0 h1 /\
-      as_matrix h1 res == S.frodo_key_encode (v b) (B.as_seq h0 a))
+    (requires fun h ->
+      B.live h a /\ B.live h res /\ B.disjoint a res)
+    (ensures fun h0 _ h1 ->
+      modifies (loc_buffer res) h0 h1 /\
+      as_matrix h1 res == S.frodo_key_encode (v b) (as_seq h0 a))
 [@"c_inline"]
 let frodo_key_encode b a res =
-  push_frame();
-
+  memset res (u16 0) (params_nbar *! params_nbar);
   let h0 = ST.get () in
-  Lib.Loops.for (size 0) params_nbar
-  (fun h1 i ->
-    B.live h1 res /\ modifies (loc_buffer res) h0 h1 /\
-    (forall (i0:size_nat{i0 < i}) (k:size_nat{k < 8}).
-      get h1 res i0 k == S.frodo_key_encode_fc (v b) (B.as_seq h0 a) i0 k) /\
-    (forall (i0:size_nat{i <= i0 /\ i0 < v params_nbar}) (k:size_nat{k < 8}).
-      get h1 res i0 k == get h0 res i0 k))
+  LSeq.eq_intro (LSeq.sub (as_seq h0 res) 0 (v params_nbar * v params_nbar)) (as_seq h0 res);
+  [@ inline_let]
+  let spec h0 = S.frodo_key_encode3 (v b) (as_seq h0 a) in
+  loop1 h0 params_nbar res spec
   (fun i ->
-    frodo_key_encode2 b a res i
-  );
-  let h1 = ST.get () in
-  S.lemma_matrix_equality_nbar (as_matrix h1 res) (S.frodo_key_encode (v b) (B.as_seq h0 a));
-  pop_frame()
+    Lib.LoopCombinators.unfold_repeati (v params_nbar) (spec h0) (as_seq h0 res) (v i);
+    let x = frodo_key_encode1 b a i in
+    frodo_key_encode2 b a i x res
+  )
 
 inline_for_extraction noextract private
 val frodo_key_decode1:
     b:size_t{0 < v b /\ v b <= 8}
-  -> a:matrix_t params_nbar params_nbar
   -> i:size_t{v i < v params_nbar}
-  -> Stack uint64
-    (requires fun h -> B.live h a)
-    (ensures fun h0 r h1 ->
-      B.live h1 a /\ modifies loc_none h0 h1 /\
-      r == S.frodo_key_decode1 (v b) (as_matrix h0 a) (v i))
-let frodo_key_decode1 b a i =
+  -> templong:uint64
+  -> res:lbytes (params_nbar *! params_nbar *! b /. size 8)
+  -> Stack unit
+    (requires fun h -> B.live h res)
+    (ensures fun h0 _ h1 ->
+      modifies (loc_buffer res) h0 h1 /\
+      as_seq h1 res == S.frodo_key_decode1 (v b) (v i) templong (as_seq h0 res))
+let frodo_key_decode1 b i templong res =
   push_frame();
-  let h0 = ST.get () in
-  let templong = create #uint64 #1 (size 1) (u64 0) in
-  let h1 = ST.get () in
-  Lib.Loops.for (size 0) (size 8)
-    (fun h2 k -> B.live h1 templong /\ B.live h2 templong /\
-      modifies (loc_buffer templong) h1 h2 /\
-      bget h2 templong 0 == S.decode_fc (v b) (as_matrix h0 a) (v i) k)
-    (fun k ->
-      let aik = mget a i k in
-      templong.(size 0) <- templong.(size 0) |. (to_u64 (dc b aik) <<. size_to_uint32 (b *! k))
-    );
-  let res = templong.(size 0) in
-  pop_frame();
-  res
-
-#set-options "--max_fuel 0"
+  let v8 = create #uint8 #8 (size 8) (u8 0) in
+  uint_to_bytes_le #_ #SEC v8 templong;
+  let tmp = sub #uint8 #8 #(v b) v8 (size 0) b in
+  update_sub res (i *! b) b tmp;
+  pop_frame()
 
 inline_for_extraction noextract private
 val frodo_key_decode2:
     b:size_t{0 < v b /\ v b <= 8}
   -> a:matrix_t params_nbar params_nbar
   -> i:size_t{v i < v params_nbar}
-  -> res:lbytes (params_nbar *! params_nbar *! b /. size 8)
-  -> Stack unit
-    (requires fun h -> B.live h a /\ B.live h res /\ B.disjoint a res)
-    (ensures fun h0 _ h1 ->
-      B.live h1 res /\ modifies (loc_buffer res) h0 h1 /\
-      B.as_seq h1 res == S.frodo_key_decode2 (v b) (as_matrix h0 a) (v i) (B.as_seq h0 res))
-let frodo_key_decode2 b a i res =
+  -> Stack uint64
+    (requires fun h -> B.live h a)
+    (ensures fun h0 r h1 ->
+      modifies loc_none h0 h1 /\
+      r == S.frodo_key_decode2 (v b) (as_matrix h0 a) (v i))
+let frodo_key_decode2 b a i =
   push_frame();
-  let templong = frodo_key_decode1 b a i in
-  let v8 = create (size 8) (u8 0) in
-  uint_to_bytes_le #U64 v8 templong;
-  let tmp = sub #uint8 #8 #(v b) v8 (size 0) b in
-  update_sub res (i *! b) b tmp;
-  pop_frame()
-
-val lemma_eq_intro_decode:
-    b:size_nat{0 < b /\ b <= 8}
-  -> s1:LSeq.lseq uint8 (v params_nbar * v params_nbar * b / 8)
-  -> s2:LSeq.lseq uint8 (v params_nbar * v params_nbar * b / 8)
-  -> Lemma
-    (requires forall (i:size_nat{i < v params_nbar}) (k:size_nat{k < b}). LSeq.index s1 (i * b + k) == LSeq.index s2 (i * b + k))
-    (ensures  s1 == s2)
-let lemma_eq_intro_decode b s1 s2 =
-  let resLen = v params_nbar * b in
-  assert (forall (i:size_nat{i < v params_nbar}) (k:size_nat{k < b}).
-    LSeq.index s1 (i * b + k) == LSeq.index s2 (i * b + k));
-  assert (forall (l:size_nat{l < resLen}). l == (l / b) * b + l % b /\ l / b < v params_nbar /\ l % b < b);
-  assert (forall (l:size_nat{l < resLen}). LSeq.index s1 l == LSeq.index s2 l);
-  LSeq.eq_intro s1 s2
+  let templong = create #uint64 #1 (size 1) (u64 0) in
+  [@ inline_let]
+  let refl h i : GTot uint64 = B.get h templong 0 in
+  [@ inline_let]
+  let footprint i = loc_buffer templong in
+  [@ inline_let]
+  let spec h0 = S.frodo_key_decode0 (v b) (as_matrix h0 a) (v i) in
+  let h0 = ST.get () in
+  assert (bget h0 templong 0 == u64 0);
+  loop h0 (size 8) S.decode_templong_t refl footprint spec
+  (fun k ->
+    Lib.LoopCombinators.unfold_repeat_gen 8 S.decode_templong_t (spec h0) (refl h0 0) (v k);
+    let aik = mget a i k in
+    templong.(size 0) <- templong.(size 0) |. (to_u64 (dc b aik) <<. (b *! k))
+  );
+  let templong = templong.(size 0) in
+  pop_frame();
+  templong
 
 val frodo_key_decode:
     b:size_t{0 < v b /\ v b <= 8}
@@ -207,15 +178,14 @@ val frodo_key_decode:
 [@"c_inline"]
 let frodo_key_decode b a res =
   let resLen = params_nbar *! params_nbar *! b /. size 8 in
+  memset res (u8 0) resLen;
   let h0 = ST.get () in
-  Lib.Loops.for (size 0) params_nbar
-    (fun h1 i ->
-      B.live h0 a /\ B.live h1 a /\ B.live h0 res /\ B.live h1 res /\
-      modifies (loc_buffer res) h0 h1 /\
-      (forall (i0:size_nat{i0 < i}) (k:size_nat{k < v b}).
-	 bget h1 res (i0 * v b + k) == S.frodo_key_decode_fc (v b) (B.as_seq h0 a) i0 k))
-    (fun i ->
-      frodo_key_decode2 b a i res
-    );
-  let h1 = ST.get () in
-  lemma_eq_intro_decode (v b) (B.as_seq h1 res) (S.frodo_key_decode (v b) (as_matrix h0 a))
+  LSeq.eq_intro (LSeq.sub (as_seq h0 res) 0 (v resLen)) (as_seq h0 res);
+  [@ inline_let]
+  let spec h0 = S.frodo_key_decode3 (v b) (as_seq h0 a) in
+  loop1 h0 params_nbar res spec
+  (fun i ->
+    Lib.LoopCombinators.unfold_repeati (v params_nbar) (spec h0) (as_seq h0 res) (v i);
+    let templong = frodo_key_decode2 b a i in
+    frodo_key_decode1 b i templong res
+  )
